Useful properties

msgequivalence.fst
@@ -140,6 +140,25 @@ let inp_hacl_to_vale #l msg =
       nat_from_intseq_le (sub msg start len) in
   inp
 
+val rem_prop_1 :
+  #l:size_t{l > 0} ->
+#lst:size_t{(l % 16 = 0 <==> lst = 16) /\ (l % 16 <> 0 <==> lst = l % 16)} ->
+#rem:size_t{rem = l - lst} ->
+v:vale_msg l ->
+Lemma (sub (inp_vale_to_hacl v) 0 rem = inp_vale_to_hacl (remove_last_block #l #lst #rem v))
+let rem_prop_1 #l #lst #rem v = ()
+
+val rem_prop_2 :
+  #l:size_t{l > 0} ->
+#lst:size_t{(l % 16 = 0 <==> lst = 16) /\ (l % 16 <> 0 <==> lst = l % 16)} ->
+#rem:size_t{rem = l - lst} ->
+i:hacl_msg l ->
+Lemma (inp_hacl_to_vale (sub i 0 rem) = remove_last_block #l #lst #rem (inp_hacl_to_vale i))
+
+let rem_prop_2 #l #lst #rem i =
+  assert (rem % 16 = 0); // required for the prover to realize this
+        ()
+
 val inp_equivalence :
   #l:size_t ->
   inp:vale_msg l ->
